Checkpoint. Finish refinesC_wcompat... Had to use strict refinement to make postconditions work out.

src/ITreeSpec/ITreeSpecDefinition.v
@@ -149,45 +149,47 @@ Defined.
 
 Create HintDb itree_spec.
 
+Local Coercion is_true : bool >-> Sortclass.
+
 Section refines.
 
   Context {E1 E2 : Type -> Type} {R1 R2 : Type}.
 
   Context (RPre : prerel E1 E2) (RPost : postrel E1 E2) (RR : R1 -> R2 -> Prop).
 
-  Inductive refinesF vclo (sim : itree_spec E1 R1 -> itree_spec E2 R2 -> Prop) : itree_spec' E1 R1 -> itree_spec' E2 R2 -> Prop := 
-  | refinesF_Ret r1 r2 : RR r1 r2 -> refinesF vclo sim (RetF r1) (RetF r2)
-  | refinesF_Tau t1 t2 : sim t1 t2 -> refinesF vclo sim (TauF t1) (TauF t2)
+  Inductive refinesF (b1 b2 : bool) vclo (sim : itree_spec E1 R1 -> itree_spec E2 R2 -> Prop) : itree_spec' E1 R1 -> itree_spec' E2 R2 -> Prop := 
+  | refinesF_Ret r1 r2 : RR r1 r2 -> refinesF b1 b2 vclo sim (RetF r1) (RetF r2)
+  | refinesF_Tau t1 t2 : sim t1 t2 -> refinesF b1 b2 vclo sim (TauF t1) (TauF t2)
 
   | refinesF_Vis {X Y} (e1 : E1 X) (e2 : E2 Y) k1 k2 :
     RPre X Y e1 e2 ->
     (forall a b, RPost X Y e1 a e2 b -> vclo sim (k1 a) (k2 b)) ->
-    refinesF vclo sim (VisF (Spec_vis e1) k1) (VisF (Spec_vis e2) k2)
+    refinesF b1 b2 vclo sim (VisF (Spec_vis e1) k1) (VisF (Spec_vis e2) k2)
 
-  | refinesF_TauL t1 ot2 : refinesF vclo sim (observe t1) ot2 -> refinesF vclo sim (TauF t1) ot2
-  | refinesF_TauR ot1 t2 : refinesF vclo sim ot1 (observe t2) -> refinesF vclo sim ot1 (TauF t2)
+  | refinesF_TauL t1 ot2 (CHECK: b1) : refinesF b1 b2 vclo sim (observe t1) ot2 -> refinesF b1 b2 vclo sim (TauF t1) ot2
+  | refinesF_TauR ot1 t2 (CHECK: b2) : refinesF b1 b2 vclo sim ot1 (observe t2) -> refinesF b1 b2 vclo sim ot1 (TauF t2)
 
-  | refinesF_forallR A ot1 k : (forall a, refinesF vclo sim ot1 (observe (k a)) ) -> refinesF vclo sim ot1 (VisF (Spec_forall A) k)
-  | refinesF_existsR A ot1 k a : refinesF vclo sim ot1 (observe (k a)) -> refinesF vclo sim ot1 (VisF (Spec_exists A) k)
-  | refinesF_forallL A ot2 k a : refinesF vclo sim (observe (k a)) ot2 -> refinesF vclo sim (VisF (Spec_forall A) k ) ot2
-  | refinesF_existsL A ot2 k : (forall a, refinesF vclo sim (observe (k a)) ot2) -> refinesF vclo sim (VisF (Spec_exists A) k) ot2
+  | refinesF_forallR A ot1 k : (forall a, refinesF b1 b2 vclo sim ot1 (observe (k a)) ) -> refinesF b1 b2 vclo sim ot1 (VisF (Spec_forall A) k)
+  | refinesF_existsR A ot1 k a : refinesF b1 b2 vclo sim ot1 (observe (k a)) -> refinesF b1 b2 vclo sim ot1 (VisF (Spec_exists A) k)
+  | refinesF_forallL A ot2 k a : refinesF b1 b2 vclo sim (observe (k a)) ot2 -> refinesF b1 b2 vclo sim (VisF (Spec_forall A) k ) ot2
+  | refinesF_existsL A ot2 k : (forall a, refinesF b1 b2 vclo sim (observe (k a)) ot2) -> refinesF b1 b2 vclo sim (VisF (Spec_exists A) k) ot2
   .
 
   Hint Constructors refinesF : itree_spec.
 
-  Definition refines_ vclo sim : itree_spec E1 R1 -> itree_spec E2 R2 -> Prop :=
-    fun t1 t2 => refinesF vclo sim (observe t1) (observe t2).
+  Definition refines_ b1 b2 vclo sim : itree_spec E1 R1 -> itree_spec E2 R2 -> Prop :=
+    fun t1 t2 => refinesF b1 b2 vclo sim (observe t1) (observe t2).
 
-  Lemma monotone_refinesF ot1 ot2 vclo vclo' sim sim'
+  Lemma monotone_refinesF ot1 ot2 b1 b2 vclo vclo' sim sim'
     (MON: monotone2 vclo)
     (LEc: vclo <3= vclo')
     (LE : sim <2= sim')
-    (IN : refinesF vclo sim ot1 ot2) : refinesF vclo' sim' ot1 ot2.
+    (IN : refinesF b1 b2 vclo sim ot1 ot2) : refinesF b1 b2 vclo' sim' ot1 ot2.
   Proof with eauto with itree_spec.
     induction IN...
   Qed.
 
-  Lemma monotone_refines_ vclo (MON: monotone2 vclo) : monotone2 (refines_ vclo).
+  Lemma monotone_refines_ b1 b2 vclo (MON: monotone2 vclo) : monotone2 (refines_ b1 b2 vclo).
   Proof. red. intros. eapply monotone_refinesF; eauto. Qed.
 
   Hint Resolve monotone_refines_ : paco.
@@ -197,7 +199,8 @@ Section refines.
 
   Hint Resolve refines_idclo_mono : paco.
 
-  Definition refines := paco2 (refines_ id) bot2.
+  Definition refines' b1 b2 := paco2 (refines_ b1 b2 id) bot2.
+  Definition refines := refines' true true.
 
 End refines.
 
